Common/CBase.v
@@ -57,20 +57,6 @@ Notation "∃' x ∈ b , P" := (exists x, x ∈ b /\ P)
   format "'[ ' '[ ' ∃' x  ∈  b ']' ,  '/' P ']'") : type_scope.
 
 
-(*** Set equivalence ***)
-
-Definition set_equiv `{SubsetEq E} : Equiv E := fun e1 e2 => e1 ⊆ e2 /\ e2 ⊆ e1.
-Infix "≡ₛ" := set_equiv (at level 70, no associativity) : stdpp_scope.
-
-Notation "(≡ₛ)" := set_equiv (only parsing) : stdpp_scope.
-Notation "( x ≡ₛ.)" := (set_equiv x) (only parsing) : stdpp_scope.
-Notation "(.≡ₛ x )" := (λ y, y ≡ₛ x) (only parsing) : stdpp_scope.
-Notation "(≢ₛ)" := (λ x y, ¬x ≡ₛ y) (only parsing) : stdpp_scope.
-Notation "x ≢ₛ y":= (¬x ≡ₛ y) (at level 70, no associativity) : stdpp_scope.
-Notation "( x ≢ₛ.)" := (λ y, x ≢ₛ y) (only parsing) : stdpp_scope.
-Notation "(.≢ₛ x )" := (λ y, y ≢ₛ x) (only parsing) : stdpp_scope.
-
-
 (*** Relations ***)
 
 Arguments clos_refl_trans {_}.
