Common/Common.v
@@ -9,6 +9,7 @@ From stdpp Require Export strings.
 From stdpp Require Export fin.
 From stdpp Require Export vector.
 From stdpp Require Export finite.
+From stdpp Require Export relations.
 Require Export Ensembles.
 
 Require Export CBase.
@@ -16,29 +17,50 @@ Require Export CBool.
 Require Export CList.
 Require Export CBitvector.
 
-(********** Utility functions **********)
+(*** Utility functions ***)
 
 (** Update a function at a specific value *)
 Definition fun_add {A B} {_: EqDecision A} (k : A) (v : B) (f : A -> B) :=
   fun x : A => if k =? x then v else f x.
 
 
-(********** Ensembles **********)
+(*** Ensembles ***)
+(* I really don't understand why this is not in stdpp *)
+(* stdpp use propset instead of Ensemble, maybe that would be better *)
 
-(* TODO: Move to stdpp *)
 Global Instance Ensemble_elem_of {A} : ElemOf A (Ensemble A) := fun x P => P x.
 
-(* TODO: Move to stdpp *)
+Global Instance Ensemble_empty {A} : Empty (Ensemble A) := fun a => False.
+
+Global Instance Ensemble_singleton {A} :
+  Singleton A (Ensemble A) := fun x y => x = y.
+
+Global Instance Ensemble_union {A} :
+  Union (Ensemble A) := fun P Q x => P x \/ Q x.
+Global Instance Ensemble_intersection {A} :
+  Intersection (Ensemble A) := fun P Q x => P x /\ Q x.
+
+Global Instance Ensemble_difference {A} :
+  Difference (Ensemble A) := fun P Q x => P x /\ ¬(Q x).
+
+
+Global Instance Ensemble_mbind : MBind Ensemble := λ A B f E b,
+    ∃'a ∈ E, b ∈ f a.
+
 Global Instance Ensemble_omap : OMap Ensemble := λ A B f E b,
     ∃'a ∈ E, f a = Some b.
 
-(* TODO: Move to stdpp *)
-Global Instance Ensemble_empty {A} : Empty (Ensemble A) := fun a => False.
 
-Definition Ensemble_from_list {A} (l : list A) : Ensemble A := fun a => a ∈ l.
+Definition Ensemble_from_set {A C} `{ElemOf A C} (c : C) : Ensemble A := fun a => a ∈ c.
+
+Global Instance Ensemble_SemiSet A : SemiSet A (Ensemble A).
+Proof. sauto l:on. Qed.
+
+Global Instance Ensemble_Set A : Set_ A (Ensemble A).
+Proof. sauto l:on. Qed.
 
 
-(********** Vectors **********)
+(*** Vectors ***)
 
 (* This is purposefully not in stdpp because Coq does not apply it automatically
    because of dependent types. This can be solved with a Hint Resolve *)
@@ -52,11 +74,13 @@ Create HintDb vec discriminated.
 #[global] Hint Rewrite @vlookup_zip_with : vec.
 
 (* There are probably lots of other lemmas to be added here,
-   I'll do case by case.
- *)
+   I'll do case by case. *)
 
 
-(********** Finite decidable quantifiers **********)
+(*** Finite decidable quantifiers ***)
+
+(* TODO maybe express with a decidable instance instead : There are consequences
+   for extraction though *)
 
 Definition fforallb {A : Type} `{Finite A} (P : A -> bool) : bool :=
   forallb P (enum A).
@@ -65,7 +89,7 @@ Lemma fforallb_brefl A `{Finite A} (P : A → bool):
   is_true (fforallb P) ↔ forall x : A, P x.
 Proof. unfold fforallb. sauto lqb:on dep:on simp+: unfold_cqual. Qed.
 #[global] Hint Rewrite fforallb_brefl : brefl.
-
+Opaque fforallb.
 
 Definition fexistsb {A : Type} `{Finite A} (P : A -> bool) : bool :=
   existsb P (enum A).
@@ -74,3 +98,4 @@ Lemma fexistsb_brefl A `{Finite A} (P : A → bool):
   is_true (fexistsb P) ↔ exists x : A, P x.
 Proof. unfold fexistsb. sauto lqb:on dep:on simp+: unfold_cqual. Qed.
 #[global] Hint Rewrite fforallb_brefl : brefl.
+Opaque fexistsb.
